crates/logic/hol/src/cbor.rs
@@ -10,7 +10,7 @@ use serde::{Deserialize, Serialize};
 
 use covalence_lib_hash::O256;
 
-use crate::{Arena, Seq};
+use crate::{Arena, Ctx, Seq};
 
 #[derive(Clone, Debug, Eq, PartialEq)]
 pub struct EncodeError(String);
@@ -66,6 +66,12 @@ pub fn seq_to_value(seq: &Seq) -> Result<Value, EncodeError> {
     to_value(seq)
 }
 pub fn seq_from_value(value: &Value) -> Result<Seq, DecodeError> {
+    from_value(value)
+}
+pub fn ctx_to_value(ctx: &Ctx) -> Result<Value, EncodeError> {
+    to_value(ctx)
+}
+pub fn ctx_from_value(value: &Value) -> Result<Ctx, DecodeError> {
     from_value(value)
 }
 pub fn import_table_to_value(table: &crate::ImportTable) -> Result<Value, EncodeError> {
